proofs/hol_light/aarch64/proofs/subroutine_signatures.ml
@@ -251,6 +251,44 @@ let subroutine_signatures = [
    ])
 );
 
+("mldsa_rej_uniform_eta2",
+  ([(*args*)
+     ("r", "int32_t[static 256]", (*is const?*)"false");
+     ("buf", "uint8_t[]", (*is const?*)"true");
+     ("buflen", "unsigned", (*is const?*)"true");
+     ("table", "uint8_t[4096]", (*is const?*)"true");
+   ],
+   "uint64_t",
+   [(* input buffers *)
+    ("buf", "buflen"(* num elems *), 1(* elem bytesize *));
+    ("table", "4096"(* num elems *), 1(* elem bytesize *));
+   ],
+   [(* output buffers *)
+    ("r", "256"(* num elems *), 4(* elem bytesize *));
+   ],
+   [(* temporary buffers *)
+   ])
+);
+
+("mldsa_rej_uniform_eta4",
+  ([(*args*)
+     ("r", "int32_t[static 256]", (*is const?*)"false");
+     ("buf", "uint8_t[]", (*is const?*)"true");
+     ("buflen", "unsigned", (*is const?*)"true");
+     ("table", "uint8_t[4096]", (*is const?*)"true");
+   ],
+   "uint64_t",
+   [(* input buffers *)
+    ("buf", "buflen"(* num elems *), 1(* elem bytesize *));
+    ("table", "4096"(* num elems *), 1(* elem bytesize *));
+   ],
+   [(* output buffers *)
+    ("r", "256"(* num elems *), 4(* elem bytesize *));
+   ],
+   [(* temporary buffers *)
+   ])
+);
+
 ("sha3_keccak_f1600",
   ([(*args*)
      ("a", "uint64_t[static 25]", (*is const?*)"false");
