proofs/hol_light/README.md
@@ -126,6 +126,8 @@ echo '1+1;;' | nc -w 5 127.0.0.1 2012
   * AArch64 pointwise multiplication-accumulation (l=5): [mld_polyvecl_pointwise_acc_montgomery_l5_aarch64_asm.S](aarch64/mldsa/mld_polyvecl_pointwise_acc_montgomery_l5_aarch64_asm.S)
   * AArch64 pointwise multiplication-accumulation (l=7): [mld_polyvecl_pointwise_acc_montgomery_l7_aarch64_asm.S](aarch64/mldsa/mld_polyvecl_pointwise_acc_montgomery_l7_aarch64_asm.S)
   * AArch64 rejection sampling: [rej_uniform_aarch64_asm.S](aarch64/mldsa/rej_uniform_aarch64_asm.S)
+  * AArch64 rejection sampling (eta=2): [rej_uniform_eta2_aarch64_asm.S](aarch64/mldsa/rej_uniform_eta2_aarch64_asm.S)
+  * AArch64 rejection sampling (eta=4): [rej_uniform_eta4_aarch64_asm.S](aarch64/mldsa/rej_uniform_eta4_aarch64_asm.S)
 - FIPS202:
   * Keccak-F1600 using lazy rotations[^HYBRID]: [keccak_f1600_x1_scalar_aarch64_asm.S](aarch64/mldsa/keccak_f1600_x1_scalar_aarch64_asm.S)
   * Keccak-F1600 using v8.4-A SHA3 instructions: [keccak_f1600_x1_v84a_aarch64_asm.S](aarch64/mldsa/keccak_f1600_x1_v84a_aarch64_asm.S)
